

Eq. (27) is the classical *replicator* (or logit) gradient. Define the simplex $\Delta^{k-1} := \{\pi \in (0, 1]^k \mid \sum_i \pi_i = 1\}$ and write $\pi_\theta = (\pi_\theta(N_1), \dots, \pi_\theta(N_k))$.

Letting $\eta \rightarrow 0$ yields the ODE

$$\dot{\pi}_i = \pi_i (A(N_i) - \langle \pi, A \rangle), \quad i = 1, \dots, k, \quad (28)$$

with $\langle \pi, A \rangle = \sum_j \pi_j A(N_j)$. Eq. (28) is the **replicator dynamics** for a fitness landscape A on Δ^{k-1} .

Consider the Kullback–Leibler divergence to the optimal pure strategy $\mathbf{e}_1 = (1, 0, \dots, 0)$,

$$V(\pi) = \sum_{i=1}^k \pi_i \ln\left(\frac{\pi_i}{e_{1,i}}\right) = -\ln \pi_1.$$

V is non-negative on Δ^{k-1} and $V(\pi) = 0$ iff $\pi = \mathbf{e}_1$.

Taking the time derivative along Eq. (28) gives

$$\frac{dV}{dt} = -\frac{\dot{\pi}_1}{\pi_1} = -(A(N_1) - \langle \pi, A \rangle) \leq 0,$$

with equality iff $\pi_1 = 1$ or $A(N_1) = \langle \pi, A \rangle$. The latter can only happen if $\pi_1 = 1$ because $A(N_1) > A(N_j)$ for $j > 1$. Hence V is a strict Lyapunov function, and \mathbf{e}_1 is the *unique* asymptotically stable equilibrium of Eq. (28). All other stationary points (mixtures over sub-optimal arms) are unstable.

For sufficiently small but fixed η (choose $\eta < \frac{1}{A^*}$, which always exists), projected gradient ascent is a *perturbed* discretisation of Eq. (28). Standard results for primal-space mirror descent imply that the discrete iterates $\pi^{(t)} \equiv \pi_{\theta(t)}$ converge almost surely to the set of asymptotically stable equilibria of the ODE, i.e. to $\{\mathbf{e}_1\}$. Therefore

$$\lim_{t \rightarrow \infty} \pi_{\theta(t)}(N_i) = \begin{cases} 1, & \text{if } i = \arg \max_j A(N_j), \\ 0, & \text{otherwise.} \end{cases}$$

Because A may attain its maximum at several arms, the limit is a deterministic policy that places all probability on *some* maximiser of A .

Thus gradient ascent on Eq. (25) converges to a deterministic policy that always selects an optimal CoT length $N^* = \arg \max_{N \in \mathcal{A}} A(N)$, completing the proof. \square

G.7 Technical Lemmas

Lemma G.1 (test point). *Let $F(x)$ be defined as*

$$F(x) = \ln\left(1 - \frac{T}{Mx}\right) + \frac{T}{Mx\left(1 - \frac{T}{Mx}\right)} + \ln\left(1 - \frac{T}{C}\right),$$

where $T, M, C \in \mathbb{R}^+$ satisfy the conditions:

- $0 < \frac{T}{C} < 0.9$,
- $0 < \frac{T}{Mx} < 1$.

Define x_0 as

$$x_0 = \frac{\sqrt{T(C-T)} + T}{M}.$$

Then, we have

$$F(x_0) < 0.$$

Proof. At $x = x_0$, note that

$$Mx_0 = \sqrt{T(C-T)} + T.$$

Thus,

$$1 - \frac{T}{Mx_0} = 1 - \frac{T}{T + \sqrt{T(C-T)}} = \frac{\sqrt{T(C-T)}}{T + \sqrt{T(C-T)}}.$$

Therefore,

$$\ln\left(1 - \frac{T}{Mx_0}\right) = \ln\left(\frac{\sqrt{T(C-T)}}{T + \sqrt{T(C-T)}}\right) = \ln\sqrt{T(C-T)} - \ln(T + \sqrt{T(C-T)}).$$

Also, observe that

$$\frac{T}{Mx_0\left(1 - \frac{T}{Mx_0}\right)} = \frac{T}{(T + \sqrt{T(C-T)})\left(\frac{\sqrt{T(C-T)}}{T + \sqrt{T(C-T)}}\right)} = \frac{T}{\sqrt{T(C-T)}} = \sqrt{\frac{T}{C-T}}.$$

It is convenient to introduce the change of variable

$$u = \sqrt{\frac{T}{C-T}},$$

so that

$$T = u^2(C-T), \quad \sqrt{T(C-T)} = u(C-T).$$

Then we have

$$T + \sqrt{T(C-T)} = u^2(C-T) + u(C-T) = u(C-T)(u+1).$$

In these terms we have:

$$\ln\sqrt{T(C-T)} = \ln[u(C-T)] = \ln u + \ln(C-T),$$

$$\ln(T + \sqrt{T(C-T)}) = \ln[u(C-T)(u+1)] = \ln u + \ln(C-T) + \ln(u+1),$$

and

$$\sqrt{\frac{T}{C-T}} = u.$$

Finally, we have

$$\ln\left(1 - \frac{T}{C}\right) = -\ln\left(\frac{C}{C-T}\right) = -\ln(u^2 + 1)$$

Thus, the function $F(x_0)$ becomes

$$F(x_0) = \ln u + \ln(C-T) - (\ln u + \ln(C-T) + \ln(u+1)) + u - \ln(u^2 + 1) \quad (29)$$

$$= -\ln(u+1) + u - \ln(u^2 + 1), \quad (30)$$

where $u = \sqrt{\frac{T}{C-T}} \in (0, 3)$. It is easy to show $F(x_0) < 0$ when $u \in (0, 3)$. □

Lemma G.2 (Estimation of the n -th Moment of the Beta Distribution). *Let $x \sim \text{Beta}(\alpha, \beta)$. Then*

$$\mathbb{E}[(1-x)^n] \leq \left(1 - \frac{\alpha}{\alpha + \beta + n - 1}\right)^n.$$

Proof.

$$\begin{aligned}
\mathbb{E}[(1-x)^n] &= \frac{1}{B(\alpha, \beta)} \int_0^1 (1-x)^n x^{\alpha-1} (1-x)^{\beta-1} dx \\
&= \frac{1}{B(\alpha, \beta)} \int_0^1 x^{\alpha-1} (1-x)^{\beta+n-1} dx \\
&= \frac{B(\alpha, \beta+n)}{B(\alpha, \beta)} \\
&= \frac{\Gamma(\alpha)\Gamma(\beta+n)}{\Gamma(\alpha+\beta+n)} \cdot \frac{\Gamma(\alpha+\beta)}{\Gamma(\alpha)\Gamma(\beta)} \\
&= \frac{\Gamma(\beta+n)}{\Gamma(\beta)} \cdot \frac{\Gamma(\alpha+\beta)}{\Gamma(\alpha+\beta+n)} \\
&= \prod_{i=0}^{n-1} \frac{\beta+i}{\alpha+\beta+i} \\
&\leq \left(\frac{\beta+n-1}{\alpha+\beta+n-1} \right)^n \\
&= \left(1 - \frac{\alpha}{\alpha+\beta+n-1} \right)^n.
\end{aligned}$$

□

H Pseudo-code of Length-filtered Vote

Algorithm 1 Length-filtered Vote

```

1: Input: Model  $f_\theta$ , Question  $q$ , Space of All Possible Answers  $A$ , Number of Total Groups  $M$ ,
   Number of Selected Groups  $K$ , Group Width  $D$ 
2: Output: Final Answer  $\hat{a}$ 
3: Sample candidates  $c_1, \dots, c_n \stackrel{i.i.d.}{\sim} f_\theta(q)$ 
4: Define  $\mathcal{A}(c)$  as the corresponding answer of candidates  $c$ .
5: Define  $p_j \in [0, 1]^{|A|}$  as the frequency of each answer in length group  $L_j$ .
6: for  $j = 1$  to  $m$  do
    $L_j = \{c_i \mid \ell(c_i) \in [D * (j-1), D * j], i = 1, \dots, n\}$ 
7:   for  $a \in A$  do
     
$$p_j[a] = \frac{\sum_{c \in L_j} \mathbb{I}(\mathcal{A}(c) = a)}{|L_j|}$$

8:   end for
9: end for
10:  $\{s_1, \dots, s_K\} = \arg \min_{S \subseteq \{1, \dots, M\}, |S|=K} \sum_{s \in S} H(p_s)$ 
11:  $\hat{a} = \arg \max_{a \in A} \sum_{c \in L_{s_1} \cup \dots \cup L_{s_K}} \mathbb{I}(\mathcal{A}(c) = a)$ 
12: return  $\hat{a}$ 

```
